TestModels/Union/src/SimpleUnionImpl.dfy
@@ -10,10 +10,22 @@ module SimpleUnionImpl refines AbstractSimpleUnionOperations  {
     predicate GetUnionEnsuresPublicly(input: GetUnionInput, output: Result<GetUnionOutput, Error>) {
         true
     }
+    predicate GetSingleValueUnionEnsuresPublicly(input: GetSingleValueUnionInput, output: Result<GetSingleValueUnionOutput, Error>) {
+        true
+    }
+
     method GetUnion ( config: InternalConfig,  input: GetUnionInput )
       returns (output: Result<GetUnionOutput, Error>)
     {
         var res := GetUnionOutput(union := input.union);
+
+        return Success(res);
+    }
+
+    method GetSingleValueUnion ( config: InternalConfig,  input: GetSingleValueUnionInput )
+      returns (output: Result<GetSingleValueUnionOutput, Error>)
+    {
+        var res := GetSingleValueUnionOutput(union := input.union);
 
         return Success(res);
     }
